Examples/Scroll/Keccak/Attributes.lean
@@ -6,4 +6,6 @@ register_simp_attr target_part_sizes_known
 register_simp_attr word_parts_known
 register_simp_attr to_cell_manager
 register_simp_attr to_decode
+register_simp_attr to_iota_s
 register_simp_attr to_os
+register_simp_attr to_s
