Examples/Scroll/Keccak/Gates/All.lean
@@ -1,3 +1,4 @@
 import Examples.Scroll.Keccak.Gates.AbsorbResult
+import Examples.Scroll.Keccak.Gates.NextRowCheck.All
 import Examples.Scroll.Keccak.Gates.Split
-import Examples.Scroll.Keccak.Gates.SplitUniform
+import Examples.Scroll.Keccak.Gates.SplitUniform.All
