Examples/Scroll/Keccak/Gates/NextRowCheck/All.lean
@@ -1,0 +1,2 @@
+import Examples.Scroll.Keccak.Gates.NextRowCheck.Gate52
+import Examples.Scroll.Keccak.Gates.NextRowCheck.Gate53
