Examples/Scroll/Keccak/Spec/All.lean
@@ -1,0 +1,7 @@
+import Examples.Scroll.Keccak.Spec.Asserts
+import Examples.Scroll.Keccak.Spec.Decode
+import Examples.Scroll.Keccak.Spec.IotaS
+import Examples.Scroll.Keccak.Spec.KeccakConstants
+import Examples.Scroll.Keccak.Spec.Os
+import Examples.Scroll.Keccak.Spec.Program
+import Examples.Scroll.Keccak.Spec.S
