Examples/Scroll/Keccak/Spec/Asserts.lean
@@ -1,0 +1,9 @@
+import Examples.Scroll.Keccak.Spec.Program
+
+namespace Keccak
+  section asserts
+    -- NOTE: assert comment says DEFAULT_KECCAK_ROWS > (NUM_BYTES_PER_WORD + 1),
+    -- but the assert states the following
+    lemma get_num_rows_per_round_assert: DEFAULT_KECCAK_ROWS > NUM_BYTES_PER_WORD := by trivial
+  end asserts
+end Keccak
