Examples/Scroll/Keccak/Spec/S.lean
@@ -1,0 +1,31 @@
+import Examples.Scroll.Keccak.Spec.Program
+
+namespace Keccak
+
+  @[to_s] lemma to_s_0_0: cell_manager c round 0 = s c round 0 0 := by unfold s; rfl
+  @[to_s] lemma to_s_0_1: cell_manager c round 1 = s c round 0 1 := by unfold s; rfl
+  @[to_s] lemma to_s_0_2: cell_manager c round 2 = s c round 0 2 := by unfold s; rfl
+  @[to_s] lemma to_s_0_3: cell_manager c round 3 = s c round 0 3 := by unfold s; rfl
+  @[to_s] lemma to_s_0_4: cell_manager c round 4 = s c round 0 4 := by unfold s; rfl
+  @[to_s] lemma to_s_1_0: cell_manager c round 5 = s c round 1 0 := by unfold s; rfl
+  @[to_s] lemma to_s_1_1: cell_manager c round 6 = s c round 1 1 := by unfold s; rfl
+  @[to_s] lemma to_s_1_2: cell_manager c round 7 = s c round 1 2 := by unfold s; rfl
+  @[to_s] lemma to_s_1_3: cell_manager c round 8 = s c round 1 3 := by unfold s; rfl
+  @[to_s] lemma to_s_1_4: cell_manager c round 9 = s c round 1 4 := by unfold s; rfl
+  @[to_s] lemma to_s_2_0: cell_manager c round 10 = s c round 2 0 := by unfold s; rfl
+  @[to_s] lemma to_s_2_1: cell_manager c round 11 = s c round 2 1 := by unfold s; rfl
+  @[to_s] lemma to_s_2_2: cell_manager c round 12 = s c round 2 2 := by unfold s; rfl
+  @[to_s] lemma to_s_2_3: cell_manager c round 13 = s c round 2 3 := by unfold s; rfl
+  @[to_s] lemma to_s_2_4: cell_manager c round 14 = s c round 2 4 := by unfold s; rfl
+  @[to_s] lemma to_s_3_0: cell_manager c round 15 = s c round 3 0 := by unfold s; rfl
+  @[to_s] lemma to_s_3_1: cell_manager c round 16 = s c round 3 1 := by unfold s; rfl
+  @[to_s] lemma to_s_3_2: cell_manager c round 17 = s c round 3 2 := by unfold s; rfl
+  @[to_s] lemma to_s_3_3: cell_manager c round 18 = s c round 3 3 := by unfold s; rfl
+  @[to_s] lemma to_s_3_4: cell_manager c round 19 = s c round 3 4 := by unfold s; rfl
+  @[to_s] lemma to_s_4_0: cell_manager c round 20 = s c round 4 0 := by unfold s; rfl
+  @[to_s] lemma to_s_4_1: cell_manager c round 21 = s c round 4 1 := by unfold s; rfl
+  @[to_s] lemma to_s_4_2: cell_manager c round 22 = s c round 4 2 := by unfold s; rfl
+  @[to_s] lemma to_s_4_3: cell_manager c round 23 = s c round 4 3 := by unfold s; rfl
+  @[to_s] lemma to_s_4_4: cell_manager c round 24 = s c round 4 4 := by unfold s; rfl
+
+end Keccak
